Fix Buffer patterns; WIP Poly1305

examples/low-level/crypto/Crypto.Symmetric.Poly1305.Spec.fst
@@ -33,7 +33,7 @@ let p_1305: p:nat{pow2 128 < p} =
 
 type elem = n:nat{n < p_1305} // elements of the field Z / p_1305 Z
 
-type word = b: seq byte {Seq.length b <= 16}
+type word = b:seq byte {Seq.length b <= 16}
 type word_16 = b:seq byte {Seq.length b = 16}
 // we only use full words for AEAD
 
@@ -69,6 +69,62 @@ val lemma_factorise: a:nat -> b:nat -> Lemma (a + a * b = a * (b + 1))
 let lemma_factorise a b = ()
 
 #reset-options "--initial_fuel 1 --max_fuel 1"
+
+val little_endian_null: len:nat{len < 16} -> Lemma
+  (little_endian (Seq.create len 0uy) == 0)
+let rec little_endian_null len =
+  if len = 0 then ()
+  else
+    begin
+    Seq.lemma_eq_intro (Seq.slice (Seq.create len 0uy) 1 len)
+		       (Seq.create (len - 1) 0uy);
+    assert (little_endian (Seq.create len 0uy) ==
+      0 + pow2 8 * little_endian (Seq.slice (Seq.create len 0uy) 1 len));
+    little_endian_null (len - 1)
+    end
+
+val little_endian_singleton: n:U8.t -> Lemma
+  (little_endian (Seq.create 1 n) == U8.v n)
+let little_endian_singleton n =
+  assert (little_endian (Seq.create 1 n) ==
+    U8.v (Seq.index (Seq.create 1 n) 0) + pow2 8 *
+    little_endian (Seq.slice (Seq.create 1 n) 1 1))
+
+val little_endian_append: w1:word -> w2:word{length w1 + length w2 <= 16} -> Lemma
+  (requires True)
+  (ensures 
+    little_endian (append w1 w2) ==
+    little_endian w1 + pow2 (8 * length w1) * little_endian w2)
+  (decreases (length w1))
+let rec little_endian_append w1 w2 =
+  if length w1 = 0 then
+    begin
+    assert_norm (pow2 (8 * 0) == 1);
+    Seq.lemma_eq_intro (append w1 w2) w2
+    end
+  else 
+    begin
+    let w1' = slice w1 1 (length w1) in
+    assert (length w1' == length w1 - 1);
+    little_endian_append w1' w2;
+    assert (index (append w1 w2) 0 == index w1 0);
+    Seq.lemma_eq_intro
+      (append w1' w2) 
+      (Seq.slice (append w1 w2) 1 (length (append w1 w2)));
+    assert (little_endian (append w1 w2) ==
+      U8.v (index w1 0) + pow2 8 * little_endian (append w1' w2));
+    assert (little_endian (append w1' w2) ==
+      little_endian w1' + pow2 (8 * length w1') * little_endian w2);
+    assert (U8.v (index w1 0) + pow2 8 * little_endian (append w1' w2) ==
+      U8.v (index w1 0) + 
+      pow2 8 * (little_endian w1' + pow2 (8 * length w1') * little_endian w2));
+    pow2_plus 8 (8 * (length w1 - 1));
+    assert (pow2 8 * pow2 (8 * length w1') == pow2 (8 * length w1));
+    assert (U8.v (index w1 0) + pow2 8 * little_endian (append w1' w2) ==
+      U8.v (index w1 0) + 
+      pow2 8 * little_endian w1' + pow2 (8 * length w1) * little_endian w2);
+    assert (U8.v (index w1 0) + pow2 8 * little_endian w1' == little_endian w1)  
+    end
 
 val lemma_little_endian_is_bounded: b:word -> Lemma
   (requires True)
@@ -107,9 +163,13 @@ let lemma_little_endian_lt_2_128 b =
 (* *            Encoding                         *)
 (* * *********************************************)
 
-let encode_16 (w:word_16) : Tot elem = pow2 128  +@  little_endian w
+let encode (w:word) : Tot elem =
+  let l = length w in
+  pow2_le_compat 128 (8 * l);
+  pow2 (8 * l) +@ little_endian w
 
 // a spec for encoding and padding, convenient for injectivity proof
+// TODO: Unused now
 let pad_0 b l = Seq.append b (Seq.create l 0uy)
 
 val encode_pad: prefix:Seq.seq elem -> txt:Seq.seq UInt8.t -> GTot (Seq.seq elem) 
@@ -118,14 +178,12 @@ let rec encode_pad prefix txt =
   let l = Seq.length txt in
   if l = 0 then prefix
   else if l < 16 then
-    begin
-    let w = pad_0 txt (16 - l) in
-    SeqProperties.snoc prefix (encode_16 w)
-    end
+    let w = txt in
+    SeqProperties.snoc prefix (encode w)
   else
     begin
     let w, txt = SeqProperties.split txt 16 in
-    let prefix = SeqProperties.snoc prefix (encode_16 w) in
+    let prefix = SeqProperties.snoc prefix (encode w) in
     encode_pad prefix txt
     end
 
@@ -208,54 +266,54 @@ let lemma_pad_0_injective b0 b1 l =
   SeqProperties.lemma_append_inj b0 (Seq.create l 0uy) b1 (Seq.create l 0uy);
   Seq.lemma_eq_intro b0 b1
 
-val lemma_encode_16_injective: w0:word_16 -> w1:word_16 -> Lemma
-  (requires (encode_16 w0 == encode_16 w1))
-  (ensures (w0 == w1))
-let lemma_encode_16_injective w0 w1 =
-  lemma_little_endian_lt_2_128 w0;
-  lemma_little_endian_lt_2_128 w1;
-  lemma_mod_plus_injective p_1305 (pow2 128) (little_endian w0) (little_endian w1);
+val lemma_encode_injective: w0:word -> w1:word -> Lemma
+  (requires (length w0 == length w1 /\ encode w0 == encode w1))
+  (ensures  (w0 == w1))
+let lemma_encode_injective w0 w1 =
+  let l = length w0 in
+  lemma_little_endian_is_bounded w0;
+  lemma_little_endian_is_bounded w1;
+  pow2_le_compat 128 (8 * l);
+  lemma_mod_plus_injective p_1305 (pow2 (8 * l))
+    (little_endian w0) (little_endian w1);
   assert (little_endian w0 == little_endian w1);
-  Seq.lemma_eq_intro (Seq.slice w0 0 16) w0;
-  Seq.lemma_eq_intro (Seq.slice w1 0 16) w1;
-  lemma_little_endian_is_injective w0 w1 16
+  Seq.lemma_eq_intro (Seq.slice w0 0 l) w0;
+  Seq.lemma_eq_intro (Seq.slice w1 0 l) w1;
+  lemma_little_endian_is_injective w0 w1 l
 
 #reset-options "--initial_fuel 1 --max_fuel 1 --initial_ifuel 0 --max_ifuel 0"
 
 val lemma_encode_pad_injective: p0:Seq.seq elem -> t0:Seq.seq UInt8.t -> p1:Seq.seq elem -> t1:Seq.seq UInt8.t -> Lemma
-  (requires
-     Seq.length t0 == Seq.length t1 /\
-     encode_pad p0 t0 == encode_pad p1 t1)
-  (ensures p0 == p1 /\ t0 == t1)
+  (requires length t0 == length t1 /\ encode_pad p0 t0 == encode_pad p1 t1)
+  (ensures  p0 == p1 /\ t0 == t1)
   (decreases (Seq.length t0))
 let rec lemma_encode_pad_injective p0 t0 p1 t1 =
   let l = Seq.length t0 in
   if l = 0 then Seq.lemma_eq_intro t0 t1
   else if l < 16 then
     begin
-    let w0 = pad_0 t0 (16 - l) in
-    let w1 = pad_0 t1 (16 - l) in
     SeqProperties.lemma_append_inj
-      p0 (Seq.create 1 (encode_16 w0))
-      p1 (Seq.create 1 (encode_16 w1));
-    lemma_index_create 1 (encode_16 w0) 0;
-    lemma_index_create 1 (encode_16 w1) 0;
-    lemma_encode_16_injective w0 w1;
-    lemma_pad_0_injective t0 t1 (16 -l)
+      p0 (Seq.create 1 (encode t0))
+      p1 (Seq.create 1 (encode t1));
+    lemma_index_create 1 (encode t0) 0;
+    lemma_index_create 1 (encode t1) 0;
+    lemma_encode_injective t0 t1
     end
   else
+    begin
     let w0, t0' = SeqProperties.split_eq t0 16 in
     let w1, t1' = SeqProperties.split_eq t1 16 in
-    let p0' = SeqProperties.snoc p0 (encode_16 w0) in
-    let p1' = SeqProperties.snoc p1 (encode_16 w1) in
+    let p0' = SeqProperties.snoc p0 (encode w0) in
+    let p1' = SeqProperties.snoc p1 (encode w1) in
     assert (encode_pad p0' t0' == encode_pad p1' t1');
     lemma_encode_pad_injective p0' t0' p1' t1';
     SeqProperties.lemma_append_inj
-      p0 (Seq.create 1 (encode_16 w0))
-      p1 (Seq.create 1 (encode_16 w1));
-    lemma_index_create 1 (encode_16 w0) 0;
-    lemma_index_create 1 (encode_16 w1) 0;
-    lemma_encode_16_injective w0 w1
+      p0 (Seq.create 1 (encode w0))
+      p1 (Seq.create 1 (encode w1));
+    lemma_index_create 1 (encode w0) 0;
+    lemma_index_create 1 (encode w1) 0;
+    lemma_encode_injective w0 w1
+    end
 
 val encode_pad_empty: prefix:Seq.seq elem -> txt:Seq.seq UInt8.t -> Lemma
   (requires Seq.length txt == 0)
@@ -263,13 +321,13 @@ val encode_pad_empty: prefix:Seq.seq elem -> txt:Seq.seq UInt8.t -> Lemma
 let encode_pad_empty prefix txt = ()
 
 val encode_pad_snoc: prefix:Seq.seq elem -> txt:Seq.seq UInt8.t -> w:word_16 -> Lemma
-  (encode_pad (SeqProperties.snoc prefix (encode_16 w)) txt ==
+  (encode_pad (SeqProperties.snoc prefix (encode w)) txt ==
    encode_pad prefix (append w txt))
 let encode_pad_snoc prefix txt w =
   Seq.lemma_len_append w txt;
   assert (16 <= Seq.length (append w txt));
   let w', txt' = SeqProperties.split (append w txt) 16 in
-  let prefix' = SeqProperties.snoc prefix (encode_16 w') in
+  let prefix' = SeqProperties.snoc prefix (encode w') in
   Seq.lemma_eq_intro w w';
   Seq.lemma_eq_intro txt txt'
 
@@ -284,7 +342,8 @@ let rec poly vs r =
   if Seq.length vs = 0 then 0
   else (poly (seq_head vs) r +@ Seq.index vs (length vs - 1)) *@ r
 
-let fix (r:word_16) (i:nat {i < 16}) m : Tot word_16 = Seq.upd r i (U8 (Seq.index r i &^ m))
+private let fix (r:word_16) (i:nat {i < 16}) m : Tot word_16 =
+  Seq.upd r i (U8 (Seq.index r i &^ m))
 
 // an abstract spec of clamping for our state invariant
 // for our polynomial-sampling assumption,
